candle/overloading/ml_kernel/ml_hol_kernel_funsProgScript.sml
@@ -6,7 +6,7 @@
   HOL functions.
 *)
 open preamble ml_translatorTheory ml_translatorLib ml_pmatchTheory patternMatchesTheory
-open astTheory libTheory evaluateTheory semanticPrimitivesTheory
+open astTheory evaluateTheory semanticPrimitivesTheory
 open ml_progLib ml_progTheory evaluateTheory
 open set_sepTheory cfTheory cfStoreTheory cfTacticsLib Satisfy
 open cfHeapsBaseTheory basisFunctionsLib
